Add hashSet lemmas

src/Std/Data/HashSet/Basic.lean
@@ -243,6 +243,17 @@ This function always merges the smaller set into the larger set, so the expected
 
 instance [BEq α] [Hashable α] : Union (HashSet α) := ⟨union⟩
 
+/--
+Computes the intersection of the given hash sets. The result will only contain entries from the first map.
+
+This function always merges the smaller set into the larger set, so the expected runtime is
+`O(min(m₁.size, m₂.size))`.
+-/
+@[inline] def inter [BEq α] [Hashable α] (m₁ m₂ : HashSet α) : HashSet α :=
+  ⟨HashMap.inter m₁.inner m₂.inner⟩
+
+instance [BEq α] [Hashable α] : Inter (HashSet α) := ⟨inter⟩
+
 section Unverified
 
 /-! We currently do not provide lemmas for the functions below. -/
